src/Bedrock/P256/Coord32.v
@@ -128,11 +128,8 @@ Local Open Scope bool_scope.
 Local Open Scope string_scope.
 Local Open Scope list_scope.
 
-Local Notation "xs $@ a" := (map.of_list_word_at a xs)
-  (at level 10, format "xs $@ a").
-Local Notation "$ n" := (match word.of_Z n return word with w => w end) (at level 9, format "$ n").
-Local Notation "p .+ n" := (word.add p (word.of_Z n)) (at level 50, format "p .+ n", left associativity).
-Local Coercion F.to_Z : F >-> Z.
+Import (notations) coqutil.Map.Memory.
+
 
 Import Specs.NotationsCustomEntry Specs.coord Specs.point.
 Local Ltac length_tac :=
